# README:
#  * The Zeitgeist ontology does not spec out what a "subject" is because we
#    use Nepomuk to describe subjects. With the convention that
#    interpretation=InformationElement and manifestation=DataObject
#    FIXME: NFO might not specify an origin for a rdfs:Resource ??



@prefix rdf: <http://www.w3.org/1999/02/22-rdf-syntax-ns#>.
@prefix rdfs: <http://www.w3.org/2000/01/rdf-schema#>.
@prefix xsd: <http://www.w3.org/2001/XMLSchema#>.
@prefix nrl: <http://www.semanticdesktop.org/ontologies/2007/08/15/nrl#>.
@prefix nao: <http://www.semanticdesktop.org/ontologies/2007/08/15/nao#>.
@prefix nie: <http://www.semanticdesktop.org/ontologies/2007/08/15/nie#>.
@prefix zg: <http://www.zeitgeist-project.com/ontologies/2010/01/27/zg#>.

zg: {
    
    zg:Event
        a rdfs:Class ;
        rdfs:subClassOf rdfs:Resource .
    
    zg:EventInterpretation
        a   rdfs:Class ;
        rdfs:comment "" ;
        rdfs:label "interpretation" ;
        rdfs:subClassOf nie:InformationElement .
    
    zg:CreateEvent
        a rdfs:Class ;
        rdfs:comment "Event type triggered when an item is created" ;
        rdfs:label "Created" ; 
        rdfs:subClassOf zg:EventInterpretation .
    
    zg:OpenEvent
        a rdfs:Class ;
        rdfs:subClassOf zg:EventInterpretation .
    
    zg:ModifyEvent
        a rdfs:Class ;
        rdfs:subClassOf zg:EventInterpretation .
    
    zg:DeleteEvent
        a rdfs:Class ;
        rdfs:subClassOf zg:EventInterpretation .
    
    zg:CloseEvent
        a rdfs:Class ;
        rdfs:subClassOf zg:EventInterpretation .
        
    zg:ReceiveEvent
        a rdfs:Class ;
        rdfs:subClassOf zg:EventInterpretation .
    
    zg:SendEvent
        a rdfs:Class ;
        rdfs:subClassOf zg:EventInterpretation .
    
    zg:EventManifestation
        a   rdfs:Class ;
        rdfs:subClassOf nie:DataObject .
    
    zg:UserActivity
        a rdfs:Class ;
        rdfs:subClassOf zg:EventManifestation .
    
    zg:HeuristicActivity
        a rdfs:Class ;
        rdfs:subClassOf zg:EventManifestation .
    
    zg:ScheduledActivity
        a rdfs:Class ;
        rdfs:subClassOf zg:EventManifestation .
    
    zg:WorldActivity
        a rdfs:Class ;
        rdfs:subClassOf zg:EventManifestation .
    
    zg:SystemNotification
        a rdfs:Class ;
        rdfs:subClassOf zg:EventManifestation .
    
    zg:eventId
        a   rdfs:Property ;
        rdfs:comment "A unique integer id assigned to an event by the logging framework when the event is first logged" ;
        rdfs:domain zg:Event ;
        rdfs:range xsd:nonNegativeInteger ;
        rdfs:label "id" ;        
        nrl:maxCardinality "1"^^xsd:nonNegativeInteger .
    
    zg:timestamp
        a   rdfs:Property ;
        rdfs:comment "Timestamp in milliseconds since the Unix Epoch" ;
        rdfs:domain zg:Event ;
        rdfs:range xsd:long ;
        rdfs:label "timestamp" ;        
        nrl:maxCardinality "1"^^xsd:nonNegativeInteger .
    
    zg:hasActor
        a   rdfs:Property ;
        rdfs:comment "The entity responsible for generating the event" ;
        rdfs:domain zg:Event ;
        rdfs:range rdfs:Resource ;
        rdfs:label "actor" ;        
        nrl:maxCardinality "1"^^xsd:nonNegativeInteger .
    
    zg:hasEventInterpretation
        a rdfs:Property ;
        rdfs:domain zg:Event ;
        rdfs:range zg:EventInterpretation ;
        nrl:maxCardinality "1"^^xsd:nonNegativeInteger ;
        rdfs:label "interpretation" ;
        rdfs:subPropertyOf nie:interpretedAs .
        
    zg:hasEventManifestation
        a rdfs:Property ;
        rdfs:domain zg:Event ;
        rdfs:range zg:EventManifestation ;
        nrl:maxCardinality "1"^^xsd:nonNegativeInteger ;
        rdfs:label "manifestation" ;
        rdfs:subPropertyOf rdfs:type .
    
    zg:hasSubject
        a rdfs:Property ;
        rdfs:domain zg:Event ;
        rdfs:range rdfs:Resource ;
        rdfs:label "subject" .
        
    zg:StorageState
        a rdf:Seq ;
        rdfs:comment "Enumeration class defining the possible values for the storage state\\n\\tof an event subject.\\n\\n\\tThe StorageState enumeration can be used to control whether or not matched\\n\\tevents must have their subjects available to the user. Fx. not including\\n\\tdeleted files, files on unplugged USB drives, files available only when\\n\\ta network is available etc." ;
        rdf:_1 zg:StorageStateNotAvailable ;
        rdf:_2 zg:StorageStateAvailable ;
        rdf:_3 zg:StorageStateAny .
        
    zg:StorageStateNotAvailable
        a rdfs:member ;
        rdfs:label "NotAvailable" ;
        rdfs:comment "The storage medium of the events subjects must not be available to the user" .
        
    zg:StorageStateAvailable
        a rdfs:member ;
        rdfs:label "Available" ;
        rdfs:comment "The storage medium of all event subjects must be immediately available to the user" .
        
    zg:StorageStateAny
        a rdfs:member ;
        rdfs:label "Any" ;
        rdfs:comment "The event subjects may or may not be available" .
        
    zg:ResultType
        a rdf:Seq ;
        rdfs:comment "An enumeration class used to define how query results should be returned\\n\\tfrom the Zeitgeist engine." ;
        rdf:_1 zg:ResultTypeMostRecentEvents ;
        rdf:_2 zg:ResultTypeLeastRecentEvents ;
        rdf:_3 zg:ResultTypeMostRecentSubjects ;
        rdf:_4 zg:ResultTypeLeastRecentSubjects ;
        rdf:_5 zg:ResultTypeMostPopularSubjects ;
        rdf:_6 zg:ResultTypeLeastPopularSubjects ;
        rdf:_7 zg:ResultTypeMostPopularActor ;
        rdf:_8 zg:ResultTypeLeastPopularActor ;
        rdf:_9 zg:ResultTypeMostRecentActor ;
        rdf:_10 zg:ResultTypeLeastRecentActor .

    zg:ResultTypeMostRecentEvents
        a rdfs:member ;
        rdfs:label "TypeMostRecentEvents" ;
        rdfs:comment "All events with the most recent events first" .

    zg:ResultTypeLeastRecentEvents
        a rdfs:member ;
        rdfs:label "LeastRecentEvents" ;
        rdfs:comment "All events with the oldest ones first" .

    zg:ResultTypeMostRecentSubjects
        a rdfs:member ;
        rdfs:label "MostRecentSubjects" ;
        rdfs:comment "One event for each subject only, ordered with the most recent events first" .

    zg:ResultTypeLeastRecentSubjects
        a rdfs:member ;
        rdfs:label "LeastRecentSubjects" ;
        rdfs:comment "One event for each subject only, ordered with oldest events first" .

    zg:ResultTypeMostPopularSubjects
        a rdfs:member ;
        rdfs:label "MostPopularSubjects" ;
        rdfs:comment "One event for each subject only, ordered by the popularity of the subject" .

    zg:ResultTypeLeastPopularSubjects
        a rdfs:member ;
        rdfs:label "LeastPopularSubjects" ;
        rdfs:comment "One event for each subject only, ordered ascendently by popularity" .

    zg:ResultTypeMostPopularActor
        a rdfs:member ;
        rdfs:label "MostPopularActor" ;
        rdfs:comment "The last event of each different actor, ordered by the popularity of the actor" .

    zg:ResultTypeLeastPopularActor
        a rdfs:member ;
        rdfs:label "LeastPopularActor" ;
        rdfs:comment "The last event of each different actor, ordered ascendently by the popularity of the actor" .

    zg:ResultTypeMostRecentActor
        a rdfs:member ;
        rdfs:label "MostRecentActor" ;
        rdfs:comment "The last event of each different actor" .

    zg:ResultTypeLeastRecentActor
        a rdfs:member ;
        rdfs:label "LeastRecentActor" ;
        rdfs:comment "The first event of each different actor" .
}


